Working version of libmGen

libmGen/libmScript.sml
@@ -1,3 +1,6 @@
+(*
+  Supporting proofs for automation
+*)
 (* Dandelion *)
 open realZeroLib floverConnTheory;
 (* CakeML & FloVer *)
@@ -13,26 +16,23 @@ Proof
   Cases_on ‘env’ >> gs[namespaceTheory.nsAppend_def, namespaceTheory.nsBind_def]
 QED
 
-Definition sem_returns_with_err_def:
-  sem_returns_with_err st envFl envReal prog progReal rv err =
-    (case evaluate st envFl [prog] of
-     | (_, Rval [FP_WordTree fp]) =>
-         (DOUBLE fp rv ∧
-          (case evaluate (empty_state with
-                    fp_state := empty_state.fp_state with
-                    <|real_sem := T; canOpt := FPScope NoOpt|>)
-                         envReal
-                    [progReal] of
-           | (_, Rval [Real r]) =>
-               real$abs (r - fp64_to_real (compress_word fp)) <= err
-           | _ => F))
-          | _ => F)
+Definition value_has_err_of_def:
+  value_has_err_of f x (rv:v) err =
+    case rv of
+    |FP_WordTree fp =>
+       (realax$abs
+        (optionGet (interp f [("x", x)]) - (fp64_to_real (compress_word fp)))
+          ≤ err)
+    | _ => F
 End
 
 Theorem theFunSpec_thm_general:
   ∀ cert lo hi exp expRat fun_v prog progReal env env2 Gamma P typeAnn A iv
-     err.
+     err ply delta v.
     getPrecondFromCert cert = P ∧
+    poly2FloVer ply = toREval exp ∧
+    ply ≠ [] ∧
+    cert.poly = ply ∧
     P 0 = (lo,hi) ∧
     exp = ratExp2realExp expRat ∧
     is64BitEval exp ∧
@@ -40,6 +40,8 @@ Theorem theFunSpec_thm_general:
     is64BitEnv Gamma ∧
     usedVars exp = LS () ∧ (* usedVars exp = { 0 } *)
     CertificateChecker exp A P Gamma = SOME typeAnn ∧
+    (∀ x. lo ≤ x ∧ x ≤ hi ⇒
+          realax$abs (optionGet (interp (cert.transc) [("x", x)]) - evalPoly ply x) ≤ delta) ∧
     FloverMapTree_find exp A = SOME (iv, err) ∧
     SOME prog = toCmlFloatProg exp ∧
     SOME progReal = toCmlRealExp expRat ∧
@@ -53,14 +55,11 @@ Theorem theFunSpec_thm_general:
       fp64_isFinite (compress_word (Fp_const fp)) /\
       DOUBLE (Fp_const fp) v ⇒
         app (p:unit ffi_proj) fun_v [v] (emp)
-          (POSTv rv.
-           &(sem_returns_with_err st
-             (env with v := nsAppend (Bind [("x0",v)] []) env.v)
-             (env with v := toRspace (nsAppend (Bind [("x0",v)] []) env.v))
-             prog progReal rv err))
+          (POSTv rv. &(value_has_err_of (cert.transc) (fp64_to_real fp) rv (delta + err)))
 Proof
   rpt strip_tac
-  >> qmatch_goalsub_abbrev_tac ‘nsAppend flEnv _’
+  >> qpat_x_assum ‘_ = env with v := nsAppend _ _’ mp_tac
+  >> qmatch_goalsub_abbrev_tac ‘nsAppend flEnv _’ >> strip_tac
   >> drule $ INST_TYPE [“:'ffi”|->“:unit”] FloVer_CakeML_sound_error
   >> rpt $ disch_then drule
   >> disch_then $ qspec_then ‘flEnv’ mp_tac >> impl_tac
@@ -71,7 +70,7 @@ Proof
   >> gs[app_def, app_basic_def] >> rpt strip_tac
   >> Q.REFINE_EXISTS_TAC ‘Val fpN’
   >> simp[evaluate_to_heap_def, evaluate_ck_def]
-  >> gs[emp_def, sem_returns_with_err_def]
+  >> gs[emp_def, value_has_err_of_def]
   >> first_x_assum $
        qspec_then ‘(st' with fp_state := st'.fp_state with
                                            <| real_sem := F; canOpt := FPScope Opt |>)’
@@ -83,6 +82,67 @@ Proof
   >> strip_tac
   >> qexists_tac ‘EMPTY’ >> qexists_tac ‘EMPTY’
   >> gs[SPLIT_def, SPLIT3_def, cond_def, DOUBLE_def]
+  >> qmatch_goalsub_abbrev_tac ‘realax$abs ( f_eval - double_eval)’
+  >> ‘f_eval - double_eval =
+      (f_eval - evalPoly ply (fp64_to_real fp)) + (evalPoly ply (fp64_to_real fp) - double_eval)’
+     by REAL_ARITH_TAC
+  >> pop_assum $ once_rewrite_tac o single
+  >> irule REAL_LE_TRANS
+  >> irule_at Any REAL_ABS_TRIANGLE
+  >> irule REAL_LE_ADD2 >> conj_tac
+  >- (
+    unabbrev_all_tac
+    >> first_x_assum irule >> gs[fpSemTheory.compress_word_def])
+  >> ‘evalPoly ply (fp64_to_real fp) = r’ suffices_by gs[]
+  >> rewrite_tac[evalPoly_Flover_eval_bisim]
+  >> gs[]
+  >> first_assum $ mp_then Any mp_tac CertificateCheckerTheory.Certificate_checking_is_sound
+  >> disch_then $ qspecl_then
+                [‘λ x. if x = 0 then SOME (fp64_to_real fp) else NONE’,
+                 ‘λ x. if x = 0 then SOME (fp64_to_real fp) else NONE’,
+                 ‘usedVars (ratExp2realExp expRat)’] mp_tac
+  >> gs[fpSemTheory.compress_word_def] >> impl_tac
+  >- (
+    gs[EnvironmentsTheory.approxEnv_def, MachineTypeTheory.computeError_pos]
+    >> ‘getValidMap Gamma (ratExp2realExp expRat) FloverMapTree_empty = Succes typeAnn’
+       by (
+          qpat_x_assum ‘CertificateChecker _ _ _ _ = _’ mp_tac
+          >> gs[CertificateCheckerTheory.CertificateChecker_def]
+          >> rpt (TOP_CASE_TAC \\ gs[]))
+    >> pop_assum $ mp_then Any mp_tac TypeValidatorTheory.getValidMap_top_correct
+    >> impl_tac >- (EVAL_TAC >> gs[])
+    >> disch_then $ mp_then Any mp_tac TypeValidatorTheory.validTypes_defined_usedVars
+    >> gs[ExpressionAbbrevsTheory.toRExpMap_def])
+  >> rpt strip_tac
+  >> first_x_assum $ mp_then Any mp_tac (INST_TYPE [“:'a”|->“:unit”] FloVer_to_CML_real_sim)
+  >> disch_then drule
+  >> disch_then $ qspec_then ‘(empty_state with
+           fp_state :=
+             empty_state.fp_state with
+             <|canOpt := FPScope NoOpt; real_sem := T|>)’ mp_tac
+  >> gs[]
+  >> disch_then $ qspecl_then [‘(λx:num. if x = 0 then SOME fp else NONE)’, ‘env’,
+                               ‘flEnv’, ‘typeAnn’, ‘vR'’,
+                               ‘domain $ usedVars expRat’] mp_tac
+  >> impl_tac
+  >- (
+    gs[] >> conj_tac
+    >- (
+      gs[real_env_rel_def, usedVars_ratExp2realExp]
+      >> unabbrev_all_tac
+      >> gs[namespaceTheory.nsLookup_def, fpSemTheory.compress_word_def])
+    >> ‘toREnv (λ x. if x = 0 then SOME fp else NONE) =
+        λ x. if x = 0 then SOME (fp64_to_real fp) else NONE’ suffices_by gs[]
+    >> gs[FUN_EQ_THM] >> rpt strip_tac >> gs[IEEE_connectionTheory.toREnv_def]
+    >> TOP_CASE_TAC >> gs[machine_ieeeTheory.fp64_to_real_def])
+  >> strip_tac
+  >> gvs[]
+  >> irule ExpressionSemanticsTheory.swap_gamma_eval_weak
+  >> first_x_assum $ irule_at Any
+  >> rpt gen_tac
+  >> Cases_on ‘e’
+  >> gs[ExpressionAbbrevsTheory.toRTMap_def]
+  >> TOP_CASE_TAC >> gs[]
 QED
 
 val _ = export_theory();
