tools/flover/Infra/README.md
@@ -1,0 +1,16 @@
+Infrastructural lemmas and formalizations for FloVer
+
+[FloverCompLib.sml](FloverCompLib.sml):
+Small changes to computeLib for FloVer
+
+[MachineTypeScript.sml](MachineTypeScript.sml):
+f machine-precision as a datatype for mixed-precision computations
+
+[RealSimpsScript.sml](RealSimpsScript.sml):
+Real-number simplification theorems
+
+[ResultsLib.sml](ResultsLib.sml):
+A monad for results used by FlOVer
+
+[ResultsScript.sml](ResultsScript.sml):
+A simple Result datatype to ease some implementations
